kg

code/ecdsap256/Hacl.Impl.P256.ECDSA.KeyGen.fst
@@ -9,33 +9,66 @@ open Lib.IntTypes
 open Lib.Buffer
 open Lib.ByteSequence
 
+open Hacl.Impl.P256.DH
+
+
+
+#set-options "--fuel 0 --ifuel 0 --z3rlimit 200"
 
 val ecdsa_p256_keyGen_privateKey: random: lbuffer uint8 (size 32)
   -> privateKey: lbuffer uint8 (size 32) -> 
   Stack bool 
-    (requires fun h -> True)
-    (ensures fun h0 _ h1 -> True)
+    (requires fun h -> live h random /\ live h privateKey /\ disjoint random privateKey)
+    (ensures fun h0 flag h1 -> modifies (loc privateKey) h0 h1 /\ (
+      let random = as_seq h0 random in 
+      let prime = Spec.ECDSAP256.Definition.prime_p256_order in 
+      if nat_from_bytes_be random > 0 && nat_from_bytes_be random < prime
+      then 
+	as_seq h1 privateKey == random /\
+	flag == true /\
+	nat_from_bytes_be (as_seq h1 privateKey) > 0 && 
+	nat_from_bytes_be (as_seq h1 privateKey) < prime 
+      else 
+	flag == false))
 
 
-let ecdsa_p256_keyGen_privateKey random result = true
+let ecdsa_p256_keyGen_privateKey random privateKey = 
+  let flag = Hacl.Impl.P256.Signature.Common.isMoreThanZeroLessThanOrder random in 
+  if flag then 
+    begin
+      copy privateKey random;
+      true 
+    end
+  else
+    false
 
 
-
-val ecdsa_p256_keyGen_publicKey_inner: privateKey: lbuffer uint8 (size 32) 
-  -> publibKey: lbuffer uint8 (size 64) -> 
-  Stack unit
-    (requires fun h -> True)
-    (ensures fun h0 _ h1 -> True)
-
-
-let ecdsa_p256_keyGen_publicKey_inner privateKey publicKey = ()
-
+open Lib.ByteSequence
 
 val ecdsa_p256_keyGen_publicKey: privateKey: lbuffer uint8 (size 32) 
-  -> publicKey: lbuffer uint8 (size 64) ->
+  -> publicKey: lbuffer uint8 (size 64) -> 
   Stack bool
-    (requires fun h -> True)
-    (ensures fun h0 _ h1 -> True)
+    (requires fun h -> live h privateKey /\ live h publicKey /\ disjoint privateKey publicKey)
+    (ensures fun h0 r h1 ->  
+      let pointX_n, pointY_n, pointZ_n = Spec.P256.secret_to_public (as_seq h0 privateKey) in
+      let pointX, pointY, flag = 
+      if Spec.P256.isPointAtInfinity (pointX_n, pointY_n, pointZ_n) then
+	nat_to_bytes_be #SEC 32 pointX_n, nat_to_bytes_be #SEC 32 pointY_n, false
+      else
+	nat_to_bytes_be 32 pointX_n, nat_to_bytes_be 32 pointY_n, true in 
+
+      modifies (loc publicKey) h0 h1 /\
+      r == flag /\
+      as_seq h1 (gsub publicKey (size 0) (size 32)) == pointX /\
+      as_seq h1 (gsub publicKey (size 32) (size 32)) == pointY
+    )
 
 
-let ecdsa_p256_keyGen_publicKey privateKey publicKey = true
+let ecdsa_p256_keyGen_publicKey privateKey publicKey = 
+  ecp256dh_i publicKey privateKey
+
+
+let ecdsa_p256_keyGen random privateKey publicKey = 
+  let flagPrivateKey = ecdsa_p256_keyGen_privateKey random privateKey in 
+  if not flagPrivateKey then false else
+  ecdsa_p256_keyGen_publicKey privateKey publicKey
