code/ecdsap256/Hacl.Impl.P256.ECDSA.KeyGen.fsti
@@ -1,0 +1,38 @@
+module Hacl.Impl.P256.ECDSA.KeyGen
+
+open FStar.HyperStack.All
+open FStar.HyperStack
+module ST = FStar.HyperStack.ST
+
+open Lib.IntTypes
+open Lib.Buffer
+open Lib.ByteSequence
+
+
+val ecdsa_p256_keyGen: random: lbuffer uint8 (size 32) 
+  -> privateKey: lbuffer uint8 (size 32) 
+  -> publicKey: lbuffer uint8 (size 64) -> 
+  Stack bool
+    (requires fun h -> live h random /\ live h privateKey /\ live h publicKey /\ 
+      disjoint privateKey random /\ disjoint privateKey publicKey)
+    (ensures fun h0 r h1 -> 
+      modifies (loc publicKey |+| loc privateKey) h0 h1 /\ (
+      let random = as_seq h0 random in 
+      let prKey = as_seq h1 privateKey in 
+      
+      let prime = Spec.ECDSAP256.Definition.prime_p256_order in 
+      
+      if nat_from_bytes_be random > 0 && nat_from_bytes_be random < prime then
+	prKey == random /\ (
+	let pointX_n, pointY_n, pointZ_n = Spec.P256.secret_to_public prKey  in
+	let pointX, pointY, flag = 
+	if Spec.P256.isPointAtInfinity (pointX_n, pointY_n, pointZ_n) then
+	  nat_to_bytes_be #SEC 32 pointX_n, nat_to_bytes_be #SEC 32 pointY_n, false
+	else
+	  nat_to_bytes_be 32 pointX_n, nat_to_bytes_be 32 pointY_n, true in 
+	
+	r == flag /\
+	as_seq h1 (gsub publicKey (size 0) (size 32)) == pointX /\
+	as_seq h1 (gsub publicKey (size 32) (size 32)) == pointY)
+    else 
+      r == false))
